

```

def basic_multivector_operations_3D():
    Print_Function()

    g3d = Ga('e*x|y|z')
    (ex, ey, ez) = g3d.mv()

    A = g3d.mv('A', 'mv')

    print('A =', A)
    print('A =', A.Fmt(2))
    print('A =', A.Fmt(3))

    print('A_{+} =', A.even())
    print('A_{-} =', A.odd())

    X = g3d.mv('X', 'vector')
    Y = g3d.mv('Y', 'vector')

    print('g_{ij} =', g3d.g)

    print('X =', X)
    print('Y =', Y)

    print('XY =', (X*Y).Fmt(2))
    print(r'X\W Y =', (X^Y).Fmt(2))
    print(r'X\cdot Y =', (X|Y).Fmt(2))
    print(r'X\times Y =', cross(X,Y).Fmt(3))
    return

```

Code Output:

$$A = A + A^x e_x + A^y e_y + A^z e_z + A^{xy} e_x \wedge e_y + A^{xz} e_x \wedge e_z + A^{yz} e_y \wedge e_z + A^{xyz} e_x \wedge e_y \wedge e_z$$

$$A = \begin{aligned} & A \\ & + A^x e_x + A^y e_y + A^z e_z \\ & + A^{xy} e_x \wedge e_y + A^{xz} e_x \wedge e_z + A^{yz} e_y \wedge e_z \\ & + A^{xyz} e_x \wedge e_y \wedge e_z \end{aligned}$$

$$A = \begin{aligned} & A \\ & + A^x e_x \\ & + A^y e_y \\ & + A^z e_z \\ & + A^{xy} e_x \wedge e_y \\ & + A^{xz} e_x \wedge e_z \\ & + A^{yz} e_y \wedge e_z \\ & + A^{xyz} e_x \wedge e_y \wedge e_z \end{aligned}$$

$$A_+ = \begin{aligned} & A \\ & + A^{xy} e_x \wedge e_y \\ & + A^{xz} e_x \wedge e_z \\ & + A^{yz} e_y \wedge e_z \end{aligned}$$

$$A_- = \begin{aligned} & A^x e_x \\ & + A^y e_y \\ & + A^z e_z \\ & + A^{xyz} e_x \wedge e_y \wedge e_z \end{aligned}$$

$$g_{ij} = \begin{bmatrix} (e_x \cdot e_x) & (e_x \cdot e_y) & (e_x \cdot e_z) \\ (e_x \cdot e_y) & (e_y \cdot e_y) & (e_y \cdot e_z) \\ (e_x \cdot e_z) & (e_y \cdot e_z) & (e_z \cdot e_z) \end{bmatrix}$$

$$X = \begin{aligned} & X^x \mathbf{e}_x \\ & + X^y \mathbf{e}_y \\ & + X^z \mathbf{e}_z \end{aligned}$$

$$Y = \begin{aligned} & Y^x \mathbf{e}_x \\ & + Y^y \mathbf{e}_y \\ & + Y^z \mathbf{e}_z \end{aligned}$$

$$XY = ((e_x \cdot e_x) X^x Y^x + (e_x \cdot e_y) X^x Y^y + (e_x \cdot e_y) X^y Y^x + (e_x \cdot e_z) X^x Y^z + (e_x \cdot e_z) X^z Y^x + (e_y \cdot e_y) X^y Y^y + (e_y \cdot e_z) X^y Y^z + (e_y \cdot e_z) X^z Y^y + (e_z \cdot e_z) X^z Y^z) \\ + (X^x Y^y - X^y Y^x) \mathbf{e}_x \wedge \mathbf{e}_y + (X^x Y^z - X^z Y^x) \mathbf{e}_x \wedge \mathbf{e}_z + (X^y Y^z - X^z Y^y) \mathbf{e}_y \wedge \mathbf{e}_z$$

$$X \wedge Y = (X^x Y^y - X^y Y^x) \mathbf{e}_x \wedge \mathbf{e}_y + (X^x Y^z - X^z Y^x) \mathbf{e}_x \wedge \mathbf{e}_z + (X^y Y^z - X^z Y^y) \mathbf{e}_y \wedge \mathbf{e}_z$$

$$X \cdot Y = (e_x \cdot e_x) X^x Y^x + (e_x \cdot e_y) X^x Y^y + (e_x \cdot e_y) X^y Y^x + (e_x \cdot e_z) X^x Y^z + (e_x \cdot e_z) X^z Y^x + (e_y \cdot e_y) X^y Y^y + (e_y \cdot e_z) X^y Y^z + (e_y \cdot e_z) X^z Y^y + (e_z \cdot e_z) X^z Y^z$$

$$\frac{(e_x \cdot e_y)(e_y \cdot e_z) X^x Y^y - (e_x \cdot e_y)(e_y \cdot e_z) X^y Y^x + (e_x \cdot e_y)(e_z \cdot e_z) X^x Y^z - (e_x \cdot e_y)(e_z \cdot e_z) X^z Y^x - (e_x \cdot e_z)(e_y \cdot e_y) X^x Y^y + (e_x \cdot e_z)(e_y \cdot e_y) X^y Y^x - (e_x \cdot e_z)(e_y \cdot e_z) X^x Y^z + (e_x \cdot e_z)(e_y \cdot e_z) X^z Y^x + (e_y \cdot e_y)(e_z \cdot e_z) X^y Y^z - (e_y \cdot e_y)(e_z \cdot e_z) X^z Y^y - (e_y \cdot e_z)^2 X^y Y^z + (e_y \cdot e_z)^2 X^z Y^y}{\sqrt{(e_x \cdot e_x)(e_y \cdot e_y)(e_z \cdot e_z) - (e_x \cdot e_x)(e_y \cdot e_z)^2 - (e_x \cdot e_y)^2(e_z \cdot e_z) + 2(e_x \cdot e_y)(e_x \cdot e_z)(e_y \cdot e_z) - (e_x \cdot e_z)^2(e_y \cdot e_y)}} \mathbf{e}_x \\ X \times Y = + \frac{-(e_x \cdot e_x)(e_y \cdot e_z) X^x Y^y + (e_x \cdot e_x)(e_y \cdot e_z) X^y Y^x - (e_x \cdot e_x)(e_z \cdot e_z) X^x Y^z + (e_x \cdot e_x)(e_z \cdot e_z) X^z Y^x + (e_x \cdot e_y)(e_x \cdot e_z) X^x Y^y - (e_x \cdot e_y)(e_x \cdot e_z) X^y Y^x - (e_x \cdot e_y)(e_z \cdot e_z) X^y Y^z + (e_x \cdot e_y)(e_z \cdot e_z) X^z Y^y + (e_x \cdot e_z)^2 X^x Y^z - (e_x \cdot e_z)^2 X^z Y^x + (e_x \cdot e_z)(e_y \cdot e_z) X^y Y^z - (e_x \cdot e_z)(e_y \cdot e_z) X^z Y^y}{\sqrt{(e_x \cdot e_x)(e_y \cdot e_y)(e_z \cdot e_z) - (e_x \cdot e_x)(e_y \cdot e_z)^2 - (e_x \cdot e_y)^2(e_z \cdot e_z) + 2(e_x \cdot e_y)(e_x \cdot e_z)(e_y \cdot e_z) - (e_x \cdot e_z)^2(e_y \cdot e_y)}} \mathbf{e}_y \\ + \frac{(e_x \cdot e_x)(e_y \cdot e_y) X^x Y^y - (e_x \cdot e_x)(e_y \cdot e_y) X^y Y^x + (e_x \cdot e_x)(e_y \cdot e_z) X^x Y^z - (e_x \cdot e_x)(e_y \cdot e_z) X^z Y^x - (e_x \cdot e_y)^2 X^x Y^y + (e_x \cdot e_y)^2 X^y Y^x - (e_x \cdot e_y)(e_x \cdot e_z) X^x Y^z + (e_x \cdot e_y)(e_x \cdot e_z) X^z Y^x + (e_x \cdot e_y)(e_y \cdot e_z) X^y Y^z - (e_x \cdot e_y)(e_y \cdot e_z) X^z Y^y - (e_x \cdot e_z)(e_y \cdot e_y) X^y Y^z + (e_x \cdot e_z)(e_y \cdot e_y) X^z Y^y}{\sqrt{(e_x \cdot e_x)(e_y \cdot e_y)(e_z \cdot e_z) - (e_x \cdot e_x)(e_y \cdot e_z)^2 - (e_x \cdot e_y)^2(e_z \cdot e_z) + 2(e_x \cdot e_y)(e_x \cdot e_z)(e_y \cdot e_z) - (e_x \cdot e_z)^2(e_y \cdot e_y)}} \mathbf{e}_z$$

```
def basic_multivector_operations_2D():
```

```
    Print_Function()
```

```
    g2d = Ga('e*x|y')
```

```
    (ex, ey) = g2d.mv()
```

```
    print('g_{ij} =', g2d.g)
```

```
    X = g2d.mv('X', 'vector')
```

```
    A = g2d.mv('A', 'spinor')
```

```
    print('X =', X)
```

```
    print('A =', A)
```

```
    print(r'X\cdot A =', (X|A).Fmt(2))
```

```
    print(r'X\lfloor A =', (X<A).Fmt(2))
```

```
    print(r'X\rfloor A =', (X>A).Fmt(2))
```

```
    return
```

Code Output:

$$g_{ij} = \begin{bmatrix} (e_x \cdot e_x) & (e_x \cdot e_y) \\ (e_x \cdot e_y) & (e_y \cdot e_y) \end{bmatrix}$$

$$X = \begin{aligned} & X^x \mathbf{e}_x \\ & + X^y \mathbf{e}_y \end{aligned}$$

$$A = \begin{aligned} & A \\ & + A^{xy} \mathbf{e}_x \wedge \mathbf{e}_y \end{aligned}$$

$$X \cdot A = -A^{xy} ((e_x \cdot e_y) X^x + (e_y \cdot e_y) X^y) \mathbf{e}_x + A^{xy} ((e_x \cdot e_x) X^x + (e_x \cdot e_y) X^y) \mathbf{e}_y$$

$$X[A = -A^{xy} ((e_x \cdot e_y) X^x + (e_y \cdot e_y) X^y) \mathbf{e}_x + A^{xy} ((e_x \cdot e_x) X^x + (e_x \cdot e_y) X^y) \mathbf{e}_y$$

$$X]A = AX^x \mathbf{e}_x + AX^y \mathbf{e}_y$$

```

def basic_multivector_operations_2D_orthogonal():
    Print_Function()
    o2d = Ga('e*x|y',g=[1,1])
    (ex,ey) = o2d.mv()
    print('g_{ii} =',o2d.g)

    X = o2d.mv('X','vector')
    A = o2d.mv('A','spinor')

    print('X =',X)
    print('A =',A)

    print('XA =',(X*A).Fmt(2))
    print(r'X\cdot A =',(X|A).Fmt(2))
    print(r'X\lfloor A =',(X<A).Fmt(2))
    print(r'X\lfloor A =',(X>A).Fmt(2))

    print('AX =',(A*X).Fmt(2))
    print(r'A\cdot X =',(A|X).Fmt(2))
    print(r'A\lfloor X =',(A<X).Fmt(2))
    print(r'A\lfloor X =',(A>X).Fmt(2))
    return

```

Code Output:

$$g_{ii} = \begin{bmatrix} 1 & 0 \\ 0 & 1 \end{bmatrix}$$

$$X = X^x e_x + X^y e_y$$

$$A = A^{xy} e_x \wedge e_y$$

$$XA = (AX^x - A^{xy}X^y) e_x + (AX^y + A^{xy}X^x) e_y$$

$$X \cdot A = -A^{xy}X^y e_x + A^{xy}X^x e_y$$

$$X|A = -A^{xy}X^y e_x + A^{xy}X^x e_y$$

$$X|A = AX^x e_x + AX^y e_y$$

$$AX = (AX^x + A^{xy}X^y) e_x + (AX^y - A^{xy}X^x) e_y$$

$$A \cdot X = A^{xy}X^y e_x - A^{xy}X^x e_y$$

$$A|X = AX^x e_x + AX^y e_y$$

$$A|X = A^{xy}X^y e_x - A^{xy}X^x e_y$$

```

def rounding_numerical_components():
    Print_Function()
    o3d = Ga('e_x e_y e_z',g=[1,1,1])
    (ex,ey,ez) = o3d.mv()

    X = 1.2*ex+2.34*ey+0.555*ez
    Y = 0.333*ex+4*ey+5.3*ez

    print('X =',X)
    print('Nga(X,2) =',Nga(X,2))
    print('XY =',X*Y)
    print('Nga(XY,2) =',Nga(X*Y,2))
    return

```

Code Output:

$$X = 1.2\mathbf{e}_x + 2.34\mathbf{e}_y + 0.555\mathbf{e}_z$$

$$Nga(X, 2) = 1.2\mathbf{e}_x + 2.3\mathbf{e}_y + 0.55\mathbf{e}_z$$

$$XY = \begin{matrix} 12.7011 \\ + 4.02078\mathbf{e}_x \wedge \mathbf{e}_y + 6.175185\mathbf{e}_x \wedge \mathbf{e}_z + 10.182\mathbf{e}_y \wedge \mathbf{e}_z \end{matrix}$$

$$Nga(XY, 2) = \begin{matrix} 13.0 \\ + 4.0\mathbf{e}_x \wedge \mathbf{e}_y + 6.2\mathbf{e}_x \wedge \mathbf{e}_z + 10.0\mathbf{e}_y \wedge \mathbf{e}_z \end{matrix}$$

```
def derivatives_in_rectangular_coordinates():
    Print_Function()
    X = (x,y,z) = symbols('x y z')
    o3d = Ga('e_x e_y e_z',g=[1,1,1],coords=X)
    (ex,ey,ez) = o3d.mv()
    grad = o3d.grad

    f = o3d.mv('f','scalar',f=True)
    A = o3d.mv('A','vector',f=True)
    B = o3d.mv('B','bivector',f=True)
    C = o3d.mv('C','mv')
    print('f =',f)
    print('A =',A)
    print('B =',B)
    print('C =',C)

    print(r'\nabla f =',grad*f)
    print(r'\nabla\cdot A =',grad|A)
    print(r'\nabla A =',grad*A)

    print(r' I(\nabla\W A) =', o3d.I()*(grad^A))
    print(r'\nabla B =',grad*B)
    print(r'\nabla\W B =',grad^B)
    print(r'\nabla\cdot B =',grad|B)
    return
```

Code Output:

$$f = f$$

$$A = A^x\mathbf{e}_x + A^y\mathbf{e}_y + A^z\mathbf{e}_z$$

$$B = B^{xy}\mathbf{e}_x \wedge \mathbf{e}_y + B^{xz}\mathbf{e}_x \wedge \mathbf{e}_z + B^{yz}\mathbf{e}_y \wedge \mathbf{e}_z$$

$$C = \begin{matrix} C \\ + C^x\mathbf{e}_x + C^y\mathbf{e}_y + C^z\mathbf{e}_z \\ + C^{xy}\mathbf{e}_x \wedge \mathbf{e}_y + C^{xz}\mathbf{e}_x \wedge \mathbf{e}_z + C^{yz}\mathbf{e}_y \wedge \mathbf{e}_z \\ + C^{xyz}\mathbf{e}_x \wedge \mathbf{e}_y \wedge \mathbf{e}_z \end{matrix}$$

$$\nabla f = \partial_x f\mathbf{e}_x + \partial_y f\mathbf{e}_y + \partial_z f\mathbf{e}_z$$

$$\nabla \cdot A = \partial_x A^x + \partial_y A^y + \partial_z A^z$$

$$\nabla A = \begin{matrix} (\partial_x A^x + \partial_y A^y + \partial_z A^z) \\ + (-\partial_y A^x + \partial_x A^y)\mathbf{e}_x \wedge \mathbf{e}_y + (-\partial_z A^x + \partial_x A^z)\mathbf{e}_x \wedge \mathbf{e}_z + (-\partial_z A^y + \partial_y A^z)\mathbf{e}_y \wedge \mathbf{e}_z \end{matrix}$$

$$-I(\nabla \wedge A) = (-\partial_z A^y + \partial_y A^z)\mathbf{e}_x + (\partial_z A^x - \partial_x A^z)\mathbf{e}_y + (-\partial_y A^x + \partial_x A^y)\mathbf{e}_z$$

$$\nabla B = \begin{matrix} (-\partial_y B^{xy} - \partial_z B^{xz})\mathbf{e}_x + (\partial_x B^{xy} - \partial_z B^{yz})\mathbf{e}_y + (\partial_x B^{xz} + \partial_y B^{yz})\mathbf{e}_z \\ + (\partial_z B^{xy} - \partial_y B^{xz} + \partial_x B^{yz})\mathbf{e}_x \wedge \mathbf{e}_y \wedge \mathbf{e}_z \end{matrix}$$

$$\nabla \wedge B = (\partial_z B^{xy} - \partial_y B^{xz} + \partial_x B^{yz})\mathbf{e}_x \wedge \mathbf{e}_y \wedge \mathbf{e}_z$$

$$\nabla \cdot B = (-\partial_y B^{xy} - \partial_z B^{xz})\mathbf{e}_x + (\partial_x B^{xy} - \partial_z B^{yz})\mathbf{e}_y + (\partial_x B^{xz} + \partial_y B^{yz})\mathbf{e}_z$$

```

def derivatives_in_spherical_coordinates():
    Print_Function()
    X = (r, th, phi) = symbols('r theta phi')
    s3d = Ga('e_r e_theta e_phi', g=[1, r**2, r**2*sin(th)**2], coords=X, norm=True)
    (er, eth, ephi) = s3d.mv()
    grad = s3d.grad

    f = s3d.mv('f', 'scalar', f=True)
    A = s3d.mv('A', 'vector', f=True)
    B = s3d.mv('B', 'bivector', f=True)

    print('f =', f)
    print('A =', A)
    print('B =', B)

    print(r'\nabla f =', grad*f)
    print(r'\nabla\cdot A =', grad|A)
    print(r' I*(\nabla\W A) =', (s3d.E()*(grad^A)).simplify())
    print(r'\nabla\W B =', grad^B)

```

Code Output:

$$f = f$$

$$A = A^r e_r + A^\theta e_\theta + A^\phi e_\phi$$

$$B = B^{r\theta} e_r \wedge e_\theta + B^{r\phi} e_r \wedge e_\phi + B^{\theta\phi} e_\theta \wedge e_\phi$$

$$\nabla f = \partial_r f e_r + \frac{\partial_\theta f}{r} e_\theta + \frac{\partial_\phi f}{r \sin(\theta)} e_\phi$$

$$\nabla \cdot A = \frac{r \partial_r A^r + 2A^r + \frac{A^\theta}{\tan(\theta)} + \partial_\theta A^\theta + \frac{\partial_\phi A^\phi}{\sin(\theta)}}{r}$$

$$-I * (\nabla \wedge A) = \frac{\frac{A^\phi}{\tan(\theta)} + \partial_\theta A^\phi - \frac{\partial_\phi A^\theta}{\sin(\theta)}}{r} e_r + \frac{-r \partial_r A^\phi - A^\phi + \frac{\partial_\phi A^r}{\sin(\theta)}}{r} e_\theta + \frac{r \partial_r A^\theta + A^\theta - \partial_\theta A^r}{r} e_\phi$$

$$\nabla \wedge B = \frac{r \partial_r B^{\theta\phi} - \frac{B^{r\phi}}{\tan(\theta)} + 2B^{\theta\phi} - \partial_\theta B^{r\phi} + \frac{\partial_\phi B^{r\theta}}{\sin(\theta)}}{r} e_r \wedge e_\theta \wedge e_\phi$$

```

def noneuclidian_distance_calculation():
    Print_Function()
    from sympy import solve, sqrt
    Fmt(1)

    g = '0 # #, # 0 #, # # 1'
    nel = Ga('X Y e', g=g)
    (X, Y, e) = nel.mv()

    print('g_{ij} =', nel.g)

    print(r'(X\W Y)^{2} =', (X^Y)*(X^Y))

    L = X^Y^e
    B = L*e # D\mathcal{L} 10.152
    Bsqr = (B*B).scalar()
    print(r'L = X\W Y\W e \T{ is a non euclidian line}')
    print('B = Le =', B)

    BeBr = B*e*B.rev()
    print(r'BeB^{\dagger} =', BeBr)
    print('B^2 =', B*B)

```

```

print( 'L^{2} =',L*L) # D&L 10.153
(s,c,Binv,M,S,C,alpha) = symbols('s c (1/B) M S C alpha')

XdotY = nel.g[0,1]
Xdote = nel.g[0,2]
Ydote = nel.g[1,2]

Bhat = Binv*B # D&L 10.154
R = c+s*Bhat # Rotor R = exp(alpha*Bhat/2)
print(r's = \f{\sinh}{\alpha/2} \T{ and } c = \f{\cosh}{\alpha/2}')
print(r'e^{\alpha B/{2\abs{B}}} =',R)

Z = R*X*R.rev() # D&L 10.155
Z.obj = expand(Z.obj)
Z.obj = Z.obj.collect([Binv,s,c,XdotY])
print(r'RXR^{\dagger}',Z.Fmt(3))
W = Z|Y # Extract scalar part of multivector
# From this point forward all calculations are with sympy scalars
#print '#Objective is to determine value of C = cosh(alpha) such that W = 0'
W = W.scalar()
print(r'W = Z\cdot Y =',W)
W = expand(W)
W = simplify(W)
W = W.collect([s*Binv])

M = 1/Bsq
W = W.subs(Binv**2,M)
W = simplify(W)
Bmag = sqrt(XdotY**2 2*XdotY*Xdote*Ydote)
W = W.collect([Binv*c*s,XdotY])

#Double angle substitutions

W = W.subs(2*XdotY**2 4*XdotY*Xdote*Ydote,2/(Binv**2))
W = W.subs(2*c*s,S)
W = W.subs(c**2,(C+1)/2)
W = W.subs(s**2,(C-1)/2)
W = simplify(W)
W = W.subs(1/Binv,Bmag)
W = expand(W)

print(r'S = \f{\sinh}{\alpha} \T{ and } C = \f{\cosh}{\alpha}')

print( 'W =',W)

Wd = collect(W,[C,S],exact=True,evaluate=False)

Wd.1 = Wd[one]
Wd.C = Wd[C]
Wd.S = Wd[S]

print(r'\T{Scalar Coefficient} =',Wd.1)
print(r'\T{Cosh Coefficient} =',Wd.C)
print(r'\T{Sinh Coefficient} =',Wd.S)

print(r'\abs{B} =',Bmag)
Wd.1 = Wd.1.subs(Bmag,1/Binv)
Wd.C = Wd.C.subs(Bmag,1/Binv)
Wd.S = Wd.S.subs(Bmag,1/Binv)

```

```

lhs = Wd_1+Wd.C*C
rhs = Wd.S*S
lhs = lhs**2
rhs = rhs**2
W = expand(lhs rhs)
W = expand(W.subs(1/Binv**2,Bmag**2))
W = expand(W.subs(S**2,C**2 1))
W = W.collect([C,C**2],evaluate=False)

a = simplify(W[C**2])
b = simplify(W[C])
c = simplify(W[one])

print(r'\T{Require } aC^{2}+bC+c = 0')

print('a =',a)
print('b =',b)
print('c =',c)

x = Symbol('x')
C = solve(a*x**2+b*x+c,x)[0]
print('b^{2} 4ac =',simplify(b**2 4*a*c))
print(r'\f{\cosh}{\alpha} = C = b/(2a) =',expand(simplify(expand(C))))
return

```

Code Output:

$$g_{ij} = \begin{bmatrix} 0 & (X \cdot Y) & (X \cdot e) \\ (X \cdot Y) & 0 & (Y \cdot e) \\ (X \cdot e) & (Y \cdot e) & 1 \end{bmatrix}$$

$$(X \wedge Y)^2 = (X \cdot Y)^2$$

$L = X \wedge Y \wedge e$ is a non-euclidian line

$$B = Le = \mathbf{X} \wedge \mathbf{Y} - (Y \cdot e) \mathbf{X} \wedge \mathbf{e} + (X \cdot e) \mathbf{Y} \wedge \mathbf{e}$$

$$BeB^\dagger = (X \cdot Y) (- (X \cdot Y) + 2(X \cdot e)(Y \cdot e)) \mathbf{e}$$

$$B^2 = (X \cdot Y) ((X \cdot Y) - 2(X \cdot e)(Y \cdot e))$$

$$L^2 = (X \cdot Y) ((X \cdot Y) - 2(X \cdot e)(Y \cdot e))$$

$$s = \sinh(\alpha/2) \text{ and } c = \cosh(\alpha/2)$$

$$e^{\alpha B/2|B|} = c + (1/B)s\mathbf{X} \wedge \mathbf{Y} - (1/B)(Y \cdot e)s\mathbf{X} \wedge \mathbf{e} + (1/B)(X \cdot e)s\mathbf{Y} \wedge \mathbf{e}$$

$$\left((1/B)^2 (X \cdot Y)^2 s^2 - 2(1/B)^2 (X \cdot Y)(X \cdot e)(Y \cdot e) s^2 + 2(1/B)(X \cdot Y)cs - 2(1/B)(X \cdot e)(Y \cdot e)cs + c^2 \right) \mathbf{X}$$

$$RXR^\dagger + 2(1/B)(X \cdot e)^2 cs\mathbf{Y}$$

$$+ 2(1/B)(X \cdot Y)(X \cdot e)s(-1/B)(X \cdot Y)s + 2(1/B)(X \cdot e)(Y \cdot e)s - c) \mathbf{e}$$

$$W = Z \cdot Y = (1/B)^2 (X \cdot Y)^3 s^2 - 4(1/B)^2 (X \cdot Y)^2 (X \cdot e)(Y \cdot e) s^2 + 4(1/B)^2 (X \cdot Y)(X \cdot e)^2 (Y \cdot e)^2 s^2 + 2(1/B)(X \cdot Y)^2 cs - 4(1/B)(X \cdot Y)(X \cdot e)(Y \cdot e)cs + (X \cdot Y)c^2$$

$$S = \sinh(\alpha) \text{ and } C = \cosh(\alpha)$$

$$W = (X \cdot Y)C - (X \cdot e)(Y \cdot e)C + (X \cdot e)(Y \cdot e) + S\sqrt{(X \cdot Y)^2 - 2(X \cdot Y)(X \cdot e)(Y \cdot e)}$$

$$\text{Scalar Coefficient} = (X \cdot e)(Y \cdot e)$$

$$\text{Cosh Coefficient} = (X \cdot Y) - (X \cdot e)(Y \cdot e)$$

$$\text{Sinh Coefficient} = \sqrt{(X \cdot Y)^2 - 2(X \cdot Y)(X \cdot e)(Y \cdot e)}$$

$$|B| = \sqrt{(X \cdot Y)^2 - 2(X \cdot Y)(X \cdot e)(Y \cdot e)}$$

$$\text{Require } aC^2 + bC + c = 0$$

$$a = (X \cdot e)^2 (Y \cdot e)^2$$

$$b = 2(X \cdot e)(Y \cdot e)((X \cdot Y) - (X \cdot e)(Y \cdot e))$$

$$c = (X \cdot Y)^2 - 2(X \cdot Y)(X \cdot e)(Y \cdot e) + (X \cdot e)^2 (Y \cdot e)^2$$

$$b^2 - 4ac = 0$$

$$\cosh(a) = C = -b/(2a) = -\frac{(X \cdot Y)}{(X \cdot e)(Y \cdot e)} + 1$$

```

def conformal_representations_of_circles_lines_spheres_and_planes():
    Print_Function()
    global n, nbar
    Fmt(1)
    g = '1 0 0 0 0,0 1 0 0 0,0 0 1 0 0,0 0 0 0 2,0 0 0 2 0'

    c3d = Ga('e_1 e_2 e_3 n \bar{n}',g=g)
    (e1,e2,e3,n,nbar) = c3d.mv()

    print('g_{ij} =',c3d.g)

    e = n+nbar
    #conformal representation of points

    A = make_vector(e1, ga=c3d) # point a = (1,0,0) A = F(a)
    B = make_vector(e2, ga=c3d) # point b = (0,1,0) B = F(b)
    C = make_vector(e1, ga=c3d) # point c = (1,0,0) C = F(c)
    D = make_vector(e3, ga=c3d) # point d = (0,0,1) D = F(d)
    X = make_vector('x',3, ga=c3d)

    print('F(a) =',A)
    print('F(b) =',B)
    print('F(c) =',C)
    print('F(d) =',D)
    print('F(x) =',X)

    print(r'a = e1, b = e2, c = e1, \T{ and } d = e3')
    print(r'A = F(a) = 1/2(a^2 n+2a nbar)\T{, etc.}')
    print(r'\T{Circle through $a$, $b$, and $c$}')
    print(r'\T{Circle: } A\W B\W C\W X = 0 =',(A^B^C^X))
    print(r'\T{Line through $a$ and $b$}')
    print(r'\T{Line : } A\W B\W n\W X = 0 =',(A^B^n^X))
    print(r'\T{Sphere through $a$, $b$, $c$, and $d$}')
    print(r'\T{Sphere: } A\W B\W C\W D\W X = 0 =,(((A^B)^C)^D)^X)
    print(r'\T{Plane through $a$, $b$, and $d$}')
    print(r'\T{Plane : } A\W B\W n\W D\W X = 0 =,(A^B^n^D^X))

    L = (A^B^e)^X

    print(r'\T{Hyperbolic \;\; Circle: } (A\W B\W e)\W X = 0',L.Fmt(3))
    return

```

Code Output:

$$g_{ij} = \begin{bmatrix} 1 & 0 & 0 & 0 & 0 \\ 0 & 1 & 0 & 0 & 0 \\ 0 & 0 & 1 & 0 & 0 \\ 0 & 0 & 0 & 0 & 2 \\ 0 & 0 & 0 & 2 & 0 \end{bmatrix}$$

$$F(a) = e_1 + \frac{1}{2}n - \frac{1}{2}\bar{n}$$

$$F(b) = \mathbf{e}_2 + \frac{1}{2}\mathbf{n} - \frac{1}{2}\bar{\mathbf{n}}$$

$$F(c) = -\mathbf{e}_1 + \frac{1}{2}\mathbf{n} - \frac{1}{2}\bar{\mathbf{n}}$$

$$F(d) = \mathbf{e}_3 + \frac{1}{2}\mathbf{n} - \frac{1}{2}\bar{\mathbf{n}}$$

$$F(x) = x_1\mathbf{e}_1 + x_2\mathbf{e}_2 + x_3\mathbf{e}_3 + \left(\frac{(x_1)^2}{2} + \frac{(x_2)^2}{2} + \frac{(x_3)^2}{2}\right)\mathbf{n} - \frac{1}{2}\bar{\mathbf{n}}$$

$$a = e1, b = e2, c = -e1, \text{ and } d = e3$$

$$A = F(a) = 1/2(a^2n + 2a - nbar), \text{ etc.}$$

Circle through a , b , and c

$$\text{Circle: } A \wedge B \wedge C \wedge X = 0 = -x_3\mathbf{e}_1 \wedge \mathbf{e}_2 \wedge \mathbf{e}_3 \wedge \mathbf{n} + x_3\mathbf{e}_1 \wedge \mathbf{e}_2 \wedge \mathbf{e}_3 \wedge \bar{\mathbf{n}} + \left(\frac{(x_1)^2}{2} + \frac{(x_2)^2}{2} + \frac{(x_3)^2}{2} - \frac{1}{2}\right)\mathbf{e}_1 \wedge \mathbf{e}_2 \wedge \mathbf{n} \wedge \bar{\mathbf{n}}$$

Line through a and b

$$\text{Line : } A \wedge B \wedge n \wedge X = 0 = -x_3\mathbf{e}_1 \wedge \mathbf{e}_2 \wedge \mathbf{e}_3 \wedge \mathbf{n} + \left(\frac{x_1}{2} + \frac{x_2}{2} - \frac{1}{2}\right)\mathbf{e}_1 \wedge \mathbf{e}_2 \wedge \mathbf{n} \wedge \bar{\mathbf{n}} + \frac{x_3}{2}\mathbf{e}_1 \wedge \mathbf{e}_3 \wedge \mathbf{n} \wedge \bar{\mathbf{n}} - \frac{x_3}{2}\mathbf{e}_2 \wedge \mathbf{e}_3 \wedge \mathbf{n} \wedge \bar{\mathbf{n}}$$

Sphere through a , b , c , and d

$$\text{Sphere: } A \wedge B \wedge C \wedge D \wedge X = 0 = \left(-\frac{(x_1)^2}{2} - \frac{(x_2)^2}{2} - \frac{(x_3)^2}{2} + \frac{1}{2}\right)\mathbf{e}_1 \wedge \mathbf{e}_2 \wedge \mathbf{e}_3 \wedge \mathbf{n} \wedge \bar{\mathbf{n}}$$

Plane through a , b , and d

$$\text{Plane : } A \wedge B \wedge n \wedge D \wedge X = 0 = \left(-\frac{x_1}{2} - \frac{x_2}{2} - \frac{x_3}{2} + \frac{1}{2}\right)\mathbf{e}_1 \wedge \mathbf{e}_2 \wedge \mathbf{e}_3 \wedge \mathbf{n} \wedge \bar{\mathbf{n}}$$

$$-x_3\mathbf{e}_1 \wedge \mathbf{e}_2 \wedge \mathbf{e}_3 \wedge \mathbf{n}$$

$$-x_3\mathbf{e}_1 \wedge \mathbf{e}_2 \wedge \mathbf{e}_3 \wedge \bar{\mathbf{n}}$$

$$\text{Hyperbolic Circle: } (A \wedge B \wedge e) \wedge X = 0 + \left(-\frac{(x_1)^2}{2} + x_1 - \frac{(x_2)^2}{2} + x_2 - \frac{(x_3)^2}{2} - \frac{1}{2}\right)\mathbf{e}_1 \wedge \mathbf{e}_2 \wedge \mathbf{n} \wedge \bar{\mathbf{n}}$$

$$+x_3\mathbf{e}_1 \wedge \mathbf{e}_3 \wedge \mathbf{n} \wedge \bar{\mathbf{n}}$$

$$-x_3\mathbf{e}_2 \wedge \mathbf{e}_3 \wedge \mathbf{n} \wedge \bar{\mathbf{n}}$$

```
def properties_of_geometric_objects():
```

```
    Print_Function()
```

```
    global n, nbar
```

```
    Fmt(1)
```

```
    g = '# # # 0 0, '+ \
        '# # # 0 0, '+ \
        '# # # 0 0, '+ \
        '0 0 0 0 2, '+ \
        '0 0 0 2 0'
```

```
    c3d = Ga('p1 p2 p3 n \bar{n}', g=g)
```

```
    (p1, p2, p3, n, nbar) = c3d.mv()
```

```
    print('g- {ij} =', c3d.g)
```

```
    P1 = F(p1)
```

```
    P2 = F(p2)
```

```
    P3 = F(p3)
```

```
    tprint('Extracting direction of line from $L = P1\W P2\W n$')
```

```
    L = P1^P2^n
```

```
    delta = (L|n)|nbar
```

```

print(r'(L\cdot n)\cdot \bar{n} =', delta)

tprint('Extracting plane of circle from $C = P1\W P2\W P3$')

C = P1^P2^P3
delta = ((C^n)|n)|nbar
print(r'((C\W n)\cdot n)\cdot \bar{n}=', delta)
print(r'(p2 p1)\W (p3 p1)=',(p2 p1)^(p3 p1))
return

```

Code Output:

$$g_{ij} = \begin{bmatrix} (p_1 \cdot p_1) & (p_1 \cdot p_2) & (p_1 \cdot p_3) & 0 & 0 \\ (p_1 \cdot p_2) & (p_2 \cdot p_2) & (p_2 \cdot p_3) & 0 & 0 \\ (p_1 \cdot p_3) & (p_2 \cdot p_3) & (p_3 \cdot p_3) & 0 & 0 \\ 0 & 0 & 0 & 0 & 2 \\ 0 & 0 & 0 & 2 & 0 \end{bmatrix}$$

Extracting direction of line from $L = P1 \wedge P2 \wedge n$

$$(L \cdot n) \cdot \bar{n} = 2\mathbf{p}_1 - 2\mathbf{p}_2$$

Extracting plane of circle from $C = P1 \wedge P2 \wedge P3$

$$((C \wedge n) \cdot n) \cdot \bar{n} = 2\mathbf{p}_1 \wedge \mathbf{p}_2 - 2\mathbf{p}_1 \wedge \mathbf{p}_3 + 2\mathbf{p}_2 \wedge \mathbf{p}_3$$

$$(p2 - p1) \wedge (p3 - p1) = \mathbf{p}_1 \wedge \mathbf{p}_2 - \mathbf{p}_1 \wedge \mathbf{p}_3 + \mathbf{p}_2 \wedge \mathbf{p}_3$$

```

def extracting_vectors_from_conformal_2_blade():
    Print_Function()
    Fmt(1)
    print(r'B = P1\W P2')

    g = '0 1 #,'+ \
        ' 1 0 #,'+ \
        '# # #'

    c2b = Ga('P1 P2 a',g=g)
    (P1,P2,a) = c2b.mv()

    print('g-{'ij} =',c2b.g)

    B = P1^P2
    Bsq = B*B
    print('B^{2} =',Bsq)
    ap = a (a^B)*B
    print(r"a' = a (a\W )B =",ap)

    Ap = ap+ap*B
    Am = ap ap*B

    print("A+ = a'+a'B =",Ap)
    print("A = a' a'B =",Am)

    print(' (A+)^{2} =',Ap*Ap)
    print(' (A)^{2} =',Am*Am)

    aB = a|B
    print(r'a\cdot B =',aB)
    return

```

Code Output:

$$B = P1 \wedge P2$$

$$g_{ij} = \begin{bmatrix} 0 & -1 & (P_1 \cdot a) \\ -1 & 0 & (P_2 \cdot a) \\ (P_1 \cdot a) & (P_2 \cdot a) & (a \cdot a) \end{bmatrix}$$

$$B^2 = 1$$

$$a' = a - (a \wedge) B = -(P_2 \cdot a) \mathbf{P}_1 - (P_1 \cdot a) \mathbf{P}_2$$

$$A+ = a' + a' B = -2(P_2 \cdot a) \mathbf{P}_1$$

$$A- = a' - a' B = -2(P_1 \cdot a) \mathbf{P}_2$$

$$(A+)^2 = 0$$

$$(A-)^2 = 0$$

$$a \cdot B = -(P_2 \cdot a) \mathbf{P}_1 + (P_1 \cdot a) \mathbf{P}_2$$

```
def reciprocal_frame_test():
    Print_Function()
    Fmt(1)
    g = '1 # #, '+ \
        '# 1 #, '+ \
        '# # 1'

    ng3d = Ga('e1 e2 e3', g=g)
    (e1, e2, e3) = ng3d.mv()

    print('g-{'ij} =', ng3d.g)

    E = e1^e2^e3
    Esq = (E*E).scalar()
    print('E =', E)
    print('E^{2} =', Esq)
    Esq_inv = 1/Esq

    E1 = (e2^e3)*E
    E2 = (1)*(e1^e3)*E
    E3 = (e1^e2)*E

    print(r'E1 = (e2\W e3)E =', E1)
    print(r'E2 = (e1\W e3)E =', E2)
    print(r'E3 = (e1\W e2)E =', E3)

    w = (E1|e2)
    w = w.expand()
    print(r'E1\cdot e2 =', w)

    w = (E1|e3)
    w = w.expand()
    print(r'E1\cdot e3 =', w)

    w = (E2|e1)
    w = w.expand()
    print(r'E2\cdot e1 =', w)

    w = (E2|e3)
    w = w.expand()
    print(r'E2\cdot e3 =', w)

    w = (E3|e1)
    w = w.expand()
    print(r'E3\cdot e1 =', w)
```

```

w = (E3|e2)
w = w.expand()
print(r'E3\cdot e2 =',w)

w = (E1|e1)
w = (w.expand()).scalar()
Esq = expand(Esq)
print(r'(E1\cdot e1)/E^{2} =', simplify(w/Esq))

w = (E2|e2)
w = (w.expand()).scalar()
print(r'(E2\cdot e2)/E^{2} =', simplify(w/Esq))

w = (E3|e3)
w = (w.expand()).scalar()
print(r'(E3\cdot e3)/E^{2} =', simplify(w/Esq))
return

```

Code Output:

$$g_{ij} = \begin{bmatrix} 1 & (e_1 \cdot e_2) & (e_1 \cdot e_3) \\ (e_1 \cdot e_2) & 1 & (e_2 \cdot e_3) \\ (e_1 \cdot e_3) & (e_2 \cdot e_3) & 1 \end{bmatrix}$$

$$E = \mathbf{e}_1 \wedge \mathbf{e}_2 \wedge \mathbf{e}_3$$

$$E^2 = (e_1 \cdot e_2)^2 - 2(e_1 \cdot e_2)(e_1 \cdot e_3)(e_2 \cdot e_3) + (e_1 \cdot e_3)^2 + (e_2 \cdot e_3)^2 - 1$$

$$E1 = (e2 \wedge e3)E = \left((e_2 \cdot e_3)^2 - 1 \right) \mathbf{e}_1 + \left((e_1 \cdot e_2) - (e_1 \cdot e_3)(e_2 \cdot e_3) \right) \mathbf{e}_2 + \left(-(e_1 \cdot e_2)(e_2 \cdot e_3) + (e_1 \cdot e_3) \right) \mathbf{e}_3$$

$$E2 = -(e1 \wedge e3)E = \left((e_1 \cdot e_2) - (e_1 \cdot e_3)(e_2 \cdot e_3) \right) \mathbf{e}_1 + \left((e_1 \cdot e_3)^2 - 1 \right) \mathbf{e}_2 + \left(-(e_1 \cdot e_2)(e_1 \cdot e_3) + (e_2 \cdot e_3) \right) \mathbf{e}_3$$

$$E3 = (e1 \wedge e2)E = \left(-(e_1 \cdot e_2)(e_2 \cdot e_3) + (e_1 \cdot e_3) \right) \mathbf{e}_1 + \left(-(e_1 \cdot e_2)(e_1 \cdot e_3) + (e_2 \cdot e_3) \right) \mathbf{e}_2 + \left((e_1 \cdot e_2)^2 - 1 \right) \mathbf{e}_3$$

$$E1 \cdot e2 = 0$$

$$E1 \cdot e3 = 0$$

$$E2 \cdot e1 = 0$$

$$E2 \cdot e3 = 0$$

$$E3 \cdot e1 = 0$$

$$E3 \cdot e2 = 0$$

$$(E1 \cdot e1)/E^2 = 1$$

$$(E2 \cdot e2)/E^2 = 1$$

$$(E3 \cdot e3)/E^2 = 1$$

```

def signature_test():
    Print_Function()

    e3d = Ga('e1 e2 e3',g=[1,1,1])
    print('g =', e3d.g)
    print(r'\T{Signature = (3,0)\:} I =', e3d.I(), '\: I^{2} =', e3d.I()*e3d.I())

    e3d = Ga('e1 e2 e3',g=[2,2,2])
    print('g =', e3d.g)
    print(r'\T{Signature = (3,0)\:} I =', e3d.I(), '\; I^{2} =', e3d.I()*e3d.I())

    sp4d = Ga('e1 e2 e3 e4',g=[1,1,1,1])
    print('g =', sp4d.g)
    print(r'\T{Signature = (1,3)\:} I =', sp4d.I(), '\: I^{2} =', sp4d.I()*sp4d.I())

```

```

sp4d = Ga('e1 e2 e3 e4',g=[2, 2, 2, 2])
print('g =', sp4d.g)
print(r'\T{Signature = (1,3)\}: I =', sp4d.I(), '\: I^{2} =', sp4d.I()*sp4d.I())

e4d = Ga('e1 e2 e3 e4',g=[1,1,1,1])
print('g =', e4d.g)
print(r'\T{Signature = (4,0)\}: I =', e4d.I(), '\: I^{2} =', e4d.I()*e4d.I())

cf3d = Ga('e1 e2 e3 e4 e5',g=[1,1,1,1,1])
print('g =', cf3d.g)
print(r'\T{Signature = (4,1)\}: I =', cf3d.I(), '\: I^{2} =', cf3d.I()*cf3d.I())

cf3d = Ga('e1 e2 e3 e4 e5',g=[2,2,2,2,2])
print('g =', cf3d.g)
print(r'\T{Signature = (4,1)\}: I =', cf3d.I(), '\: I^{2} =', cf3d.I()*cf3d.I())

return

```

Code Output:

$$g = \begin{bmatrix} 1 & 0 & 0 \\ 0 & 1 & 0 \\ 0 & 0 & 1 \end{bmatrix}$$

$$\text{Signature} = (3,0) \quad I = \mathbf{e}_1 \wedge \mathbf{e}_2 \wedge \mathbf{e}_3 \quad I^2 = -1$$

$$g = \begin{bmatrix} 2 & 0 & 0 \\ 0 & 2 & 0 \\ 0 & 0 & 2 \end{bmatrix}$$

$$r\text{Signature} = (3,0) \quad I = \frac{\sqrt{2}}{4} \mathbf{e}_1 \wedge \mathbf{e}_2 \wedge \mathbf{e}_3 \quad I^2 = -1$$

$$g = \begin{bmatrix} 1 & 0 & 0 & 0 \\ 0 & -1 & 0 & 0 \\ 0 & 0 & -1 & 0 \\ 0 & 0 & 0 & -1 \end{bmatrix}$$

$$\text{Signature} = (1,3) \quad I = \mathbf{e}_1 \wedge \mathbf{e}_2 \wedge \mathbf{e}_3 \wedge \mathbf{e}_4 \quad I^2 = -1$$

$$g = \begin{bmatrix} 2 & 0 & 0 & 0 \\ 0 & -2 & 0 & 0 \\ 0 & 0 & -2 & 0 \\ 0 & 0 & 0 & -2 \end{bmatrix}$$

$$\text{Signature} = (1,3) \quad I = \frac{1}{4} \mathbf{e}_1 \wedge \mathbf{e}_2 \wedge \mathbf{e}_3 \wedge \mathbf{e}_4 \quad I^2 = -1$$

$$g = \begin{bmatrix} 1 & 0 & 0 & 0 \\ 0 & 1 & 0 & 0 \\ 0 & 0 & 1 & 0 \\ 0 & 0 & 0 & 1 \end{bmatrix}$$

$$\text{Signature} = (4,0) \quad I = \mathbf{e}_1 \wedge \mathbf{e}_2 \wedge \mathbf{e}_3 \wedge \mathbf{e}_4 \quad I^2 = 1$$

$$g = \begin{bmatrix} 1 & 0 & 0 & 0 & 0 \\ 0 & 1 & 0 & 0 & 0 \\ 0 & 0 & 1 & 0 & 0 \\ 0 & 0 & 0 & 1 & 0 \\ 0 & 0 & 0 & 0 & -1 \end{bmatrix}$$

$$\text{Signature} = (4,1) \quad I = \mathbf{e}_1 \wedge \mathbf{e}_2 \wedge \mathbf{e}_3 \wedge \mathbf{e}_4 \wedge \mathbf{e}_5 \quad I^2 = -1$$

$$g = \begin{bmatrix} 2 & 0 & 0 & 0 & 0 \\ 0 & 2 & 0 & 0 & 0 \\ 0 & 0 & 2 & 0 & 0 \\ 0 & 0 & 0 & 2 & 0 \\ 0 & 0 & 0 & 0 & -2 \end{bmatrix}$$

$$\text{Signature} = (4,1) \quad I = \frac{\sqrt{2}}{8} \mathbf{e}_1 \wedge \mathbf{e}_2 \wedge \mathbf{e}_3 \wedge \mathbf{e}_4 \wedge \mathbf{e}_5 \quad I^2 = -1$$

```
def Fmt_test():
    Print_Function()

    e3d = Ga('e1 e2 e3',g=[1,1,1])

    v = e3d.mv('v','vector')
    B = e3d.mv('B','bivector')
    M = e3d.mv('M','mv')

    Fmt(2)

    tprint('Global $Fmt = 2$')

    print('v =',v)
    print('B =',B)
    print('M =',M)

    tprint('Using $.Fmt()$ Function')

    print('v.Fmt(3) =',v.Fmt(3))
    print('B.Fmt(3) =',B.Fmt(3))
    print('M.Fmt(2) =',M.Fmt(2))
    print('M.Fmt(1) =',M.Fmt(1))

    print('Global $Fmt = 1$')

    Fmt(1)

    print('v =',v)
    print('B =',B)
    print('M =',M)

    return
```

Code Output:

Global $Fmt = 2$

$$v = v^1 \mathbf{e}_1 + v^2 \mathbf{e}_2 + v^3 \mathbf{e}_3$$

$$B = B^{12} \mathbf{e}_1 \wedge \mathbf{e}_2 + B^{13} \mathbf{e}_1 \wedge \mathbf{e}_3 + B^{23} \mathbf{e}_2 \wedge \mathbf{e}_3$$

M

$$M = \begin{aligned} &+ M^1 \mathbf{e}_1 + M^2 \mathbf{e}_2 + M^3 \mathbf{e}_3 \\ &+ M^{12} \mathbf{e}_1 \wedge \mathbf{e}_2 + M^{13} \mathbf{e}_1 \wedge \mathbf{e}_3 + M^{23} \mathbf{e}_2 \wedge \mathbf{e}_3 \\ &+ M^{123} \mathbf{e}_1 \wedge \mathbf{e}_2 \wedge \mathbf{e}_3 \end{aligned}$$

Using $.Fmt()$ Function

$$v.Fmt(3) = \begin{aligned} &v^1 \mathbf{e}_1 \\ &+ v^2 \mathbf{e}_2 \\ &+ v^3 \mathbf{e}_3 \end{aligned}$$

$$B.Fmt(3) = B^{12}\mathbf{e}_1 \wedge \mathbf{e}_2 + B^{13}\mathbf{e}_1 \wedge \mathbf{e}_3 + B^{23}\mathbf{e}_2 \wedge \mathbf{e}_3$$

$$M.Fmt(2) = M + M^1\mathbf{e}_1 + M^2\mathbf{e}_2 + M^3\mathbf{e}_3 + M^{12}\mathbf{e}_1 \wedge \mathbf{e}_2 + M^{13}\mathbf{e}_1 \wedge \mathbf{e}_3 + M^{23}\mathbf{e}_2 \wedge \mathbf{e}_3 + M^{123}\mathbf{e}_1 \wedge \mathbf{e}_2 \wedge \mathbf{e}_3$$

$$M.Fmt(1) = M + M^1\mathbf{e}_1 + M^2\mathbf{e}_2 + M^3\mathbf{e}_3 + M^{12}\mathbf{e}_1 \wedge \mathbf{e}_2 + M^{13}\mathbf{e}_1 \wedge \mathbf{e}_3 + M^{23}\mathbf{e}_2 \wedge \mathbf{e}_3 + M^{123}\mathbf{e}_1 \wedge \mathbf{e}_2 \wedge \mathbf{e}_3$$

$$GlobalFmt = 1$$

$$v = v^1\mathbf{e}_1 + v^2\mathbf{e}_2 + v^3\mathbf{e}_3$$

$$B = B^{12}\mathbf{e}_1 \wedge \mathbf{e}_2 + B^{13}\mathbf{e}_1 \wedge \mathbf{e}_3 + B^{23}\mathbf{e}_2 \wedge \mathbf{e}_3$$

$$M = M + M^1\mathbf{e}_1 + M^2\mathbf{e}_2 + M^3\mathbf{e}_3 + M^{12}\mathbf{e}_1 \wedge \mathbf{e}_2 + M^{13}\mathbf{e}_1 \wedge \mathbf{e}_3 + M^{23}\mathbf{e}_2 \wedge \mathbf{e}_3 + M^{123}\mathbf{e}_1 \wedge \mathbf{e}_2 \wedge \mathbf{e}_3$$